Gt3/HasTy/Regular.lean
@@ -61,9 +61,11 @@ theorem Ctx.JEq.cmp {Γ A a b} (h : JEq Γ A a b) : Cmp Γ A a b := by induction
         | assumption
         | intros; apply HasTy.cast_top_symm' <;> apply_assumption; assumption
         | intros; apply HasTy.cast_top_symm₂ <;> apply_assumption <;> assumption
-        | apply Ctx.JEq.lst_cf_cast_lhs <;> first | assumption | apply Ctx.JEq.lhs_is_ty; assumption
         | apply Ctx.HasTy.lst_cf_cast <;> assumption
         | apply Ctx.HasTy.cast' <;> assumption
+        | apply Ctx.JEq.lst_cf_cast_lhs <;> first | assumption
+                                                  | apply Ctx.JEq.lhs_is_ty; assumption
+                                                  | apply Ctx.JEq.fst' <;> assumption
       · first
         | apply TyEq.symm; apply JEq.ty_eq; assumption
         | (ty_eq_constructor'
